STLC_SuccNat/STLC_SuccNat.v
@@ -401,3 +401,33 @@ Proof.
    eapply multi_step.
      apply ST_Succ; eauto.  auto.
 Qed.
+
+Lemma multistep_cons1 : forall t1 t2 t3,
+  multi step t1 t2 -> multi step (cons t1 t3) (cons t2 t3).
+Proof.
+  intros t1 t2 t3 Hms. induction Hms.
+    apply multi_refl.
+    eapply multi_step.
+      apply ST_Cons1; eauto. auto.
+Qed.
+
+Lemma multistep_cons2 : forall v1 t2 t3,
+  value v1 ->
+  multi step t2 t3 ->
+  multi step (cons v1 t2) (cons v1 t3).
+Proof.
+  intros v1 t2 t3 Hv Hms. induction Hms.
+    apply multi_refl.
+    eapply multi_step.
+      apply ST_Cons2; eauto. auto.
+Qed.
+
+Lemma multistep_case1 : forall x y t1 t2 tnil tcons,
+  multi step t1 t2 -> multi step (case t1 tnil x y tcons)
+                                 (case t2 tnil x y tcons).
+Proof.
+  intros x y t1 t2 tnil tcons Hms. induction Hms.
+    apply multi_refl.
+    eapply multi_step.
+      apply ST_Case1; eauto. auto.
+Qed.
